lib/WPProofs.v
@@ -895,12 +895,12 @@ Section WPProofs.
 
   Lemma wp_op'_size:
     forall (c: bctx) si (o: P4A.op Hdr_sz) n phi m phi',
-      WP.wp_op' (c:=c) si o (P4A.op_size o + n, phi) = (m, phi') ->
+      WP.wp_op' (c:=c) a si o (P4A.op_size o + n, phi) = (m, phi') ->
       m = n.
   Proof.
     induction o; cbn; intros.
     - congruence.
-    - destruct (WP.wp_op' si o2 (P4A.op_size o1 + P4A.op_size o2 + n, phi)) eqn:?.
+    - destruct (WP.wp_op' a si o2 (P4A.op_size o1 + P4A.op_size o2 + n, phi)) eqn:?.
       replace (P4A.op_size o1 + P4A.op_size o2 + n)
         with (P4A.op_size o2 + (P4A.op_size o1 + n))
         in *
@@ -916,7 +916,7 @@ Section WPProofs.
 
   Lemma wp_op'_seq:
     forall (c: bctx) (o1: P4A.op Hdr_sz) (o2: P4A.op Hdr_sz) si phi,
-      WP.wp_op' (c:=c) si (P4A.OpSeq o1 o2) phi = WP.wp_op' si o1 (WP.wp_op' si o2 phi).
+      WP.wp_op' (c:=c) a si (P4A.OpSeq o1 o2) phi = WP.wp_op' a si o1 (WP.wp_op' a si o2 phi).
   Proof.
     induction o1; intros; simpl;
       repeat match goal with
@@ -929,12 +929,12 @@ Section WPProofs.
 
   Lemma wp_op'_mono:
     forall (c: bctx) si (o: P4A.op Hdr_sz) n phi,
-      fst (WP.wp_op' (c:=c) si o (n, phi)) <= n.
+      fst (WP.wp_op' (c:=c) a si o (n, phi)) <= n.
   Proof.
     induction o; simpl.
     - Lia.lia.
     - intros.
-      destruct (WP.wp_op' si o2 _) as [m psi] eqn:?.
+      destruct (WP.wp_op' a si o2 _) as [m psi] eqn:?.
       specialize (IHo2 n phi).
       specialize (IHo1 m psi).
       rewrite Heqp in *.
@@ -1170,12 +1170,42 @@ Section WPProofs.
     reflexivity.
   Qed.
 
+  Lemma quantifier_subst_left:
+    forall c b1 b2 (buf1: n_tuple bool b1) (buf2: n_tuple bool b2) st1 st2 lhs rhs (buf1': n_tuple bool _) phi valu,
+    interp_store_rel
+    (BRForAll
+       (BRImpl
+          (BREq (BEVar Hdr (BVarTop c (Hdr_sz lhs))) (expr_to_bit_expr Left rhs))
+          (sr_subst (weaken_store_rel a (Hdr_sz lhs) phi)
+             (BEVar Hdr (BVarTop c (Hdr_sz lhs)))
+             (BEHdr (BCSnoc c (Hdr_sz lhs)) Left (ConfRel.P4A.HRVar lhs))))) valu
+    buf1 buf2 st1 st2 <->
+  interp_store_rel (a:=a) phi valu buf1 buf2
+    (P4A.eval_op Hdr Hdr_sz st1 (P4A.OpAsgn lhs rhs) buf1') st2.
+  Proof.
+  Admitted.
+
+  Lemma quantifier_subst_right:
+    forall c b1 b2 (buf1: n_tuple bool b1) (buf2: n_tuple bool b2) st1 st2 lhs rhs (buf2':  n_tuple bool _) phi valu,
+  interp_store_rel
+    (BRForAll
+       (BRImpl
+          (BREq (BEVar Hdr (BVarTop c (Hdr_sz lhs))) (expr_to_bit_expr Right rhs))
+          (sr_subst (weaken_store_rel a (Hdr_sz lhs) phi)
+             (BEVar Hdr (BVarTop c (Hdr_sz lhs)))
+             (BEHdr (BCSnoc c (Hdr_sz lhs)) Right (ConfRel.P4A.HRVar lhs)))))
+    valu buf1 buf2 st1 st2 <->
+  interp_store_rel (a:=a) phi valu buf1 buf2 st1
+    (P4A.eval_op Hdr Hdr_sz st2 (P4A.OpAsgn lhs rhs) buf2').
+  Proof.
+  Admitted.
+
   Lemma wp_op'_spec_l:
     forall c (valu: bval c) (o: P4A.op Hdr_sz) n m phi st1
       (buf1: n_tuple bool (n + P4A.op_size o + m)) (buf1': n_tuple bool (P4A.op_size o)) len2 (buf2: n_tuple bool len2) st2,
       buf1' ~= n_tuple_take_n (P4A.op_size o) (n_tuple_skip_n n buf1) ->
       interp_store_rel (a:=a)
-                       (snd (WP.wp_op' Left o (n + P4A.op_size o, phi)))
+                       (snd (WP.wp_op' a Left o (n + P4A.op_size o, phi)))
                        valu
                        buf1
                        buf2
@@ -1198,7 +1228,7 @@ Section WPProofs.
       reflexivity.
     - intros.
       rewrite wp_op'_seq.
-      destruct (wp_op' Left o2 _) as [n' phi'] eqn:?.
+      destruct (wp_op' a Left o2 _) as [n' phi'] eqn:?.
       simpl in Heqp.
       replace (n + (P4A.op_size o1 + P4A.op_size o2)) with (P4A.op_size o2 + (n + P4A.op_size o1))
         in Heqp by Lia.lia.
@@ -1334,10 +1364,7 @@ Section WPProofs.
       {
         now apply vbits_inv in H0.
       }
-      rewrite sr_subst_hdr_left; eauto.
-      autorewrite with eval_op.
-      rewrite Heqv.
-      reflexivity.
+      apply quantifier_subst_left.
   Qed.
 
   Lemma wp_op'_spec_r:
@@ -1345,7 +1372,7 @@ Section WPProofs.
       (buf2: n_tuple bool (n + P4A.op_size o + m)) (buf2': n_tuple bool (P4A.op_size o)) len1 (buf1: n_tuple bool len1) st1,
       buf2' ~= n_tuple_take_n (P4A.op_size o) (n_tuple_skip_n n buf2) ->
       interp_store_rel (a:=a)
-                       (snd (WP.wp_op' Right o (n + P4A.op_size o, phi)))
+                       (snd (WP.wp_op' a Right o (n + P4A.op_size o, phi)))
                        valu
                        buf1
                        buf2
@@ -1368,7 +1395,7 @@ Section WPProofs.
       reflexivity.
     - intros.
       rewrite wp_op'_seq.
-      destruct (wp_op' Right o2 _) as [n' phi'] eqn:?.
+      destruct (wp_op' a Right o2 _) as [n' phi'] eqn:?.
       simpl P4A.op_size in Heqp.
       replace (n + (P4A.op_size o1 + P4A.op_size o2)) with (P4A.op_size o2 + (n + P4A.op_size o1))
         in Heqp by Lia.lia.
@@ -1502,10 +1529,7 @@ Section WPProofs.
       {
         now apply vbits_inv in H0.
       }
-      rewrite sr_subst_hdr_right; eauto.
-      autorewrite with eval_op.
-      rewrite Heqv.
-      reflexivity.
+      apply quantifier_subst_right.
   Qed.
 
   Lemma in_interp_tpairs:
@@ -2426,72 +2450,10 @@ Section WPProofs.
     reflexivity.
   Qed.
 
-  Lemma weaken_bvar_interp:
-    forall (c: bctx) (n: nat) (valu: bval c) (bits: n_tuple bool n) (b: bvar c),
-    interp_bvar ((valu, bits): bval (BCSnoc c n)) (weaken_bvar n b) ~= interp_bvar valu b.
-  Proof.
-    destruct b, valu; simpl; autorewrite with interp_bvar; reflexivity.
-  Qed.
-
-  Lemma weaken_expr_interp:
-    forall c n e (valu: bval c) (bits: n_tuple bool n) l1 l2 (buf1: n_tuple bool l1) (buf2: n_tuple bool l2) store1 store2,
-      interp_bit_expr (weaken_bit_expr n e) (valu, bits) buf1 buf2 store1 store2 ~=
-      interp_bit_expr (a:=a) e valu buf1 buf2 store1 store2.
-  Proof.
-    induction e; intros; simpl; autorewrite with interp_bit_expr in *.
-    - auto.
-    - destruct a0; autorewrite with interp_bit_expr; auto.
-    - destruct a0; simpl; auto.
-    - apply weaken_bvar_interp.
-    - set (v1 := interp_bit_expr (weaken_bit_expr n e) (valu, bits) buf1 buf2 store1
-                               store2).
-      set (v2 := interp_bit_expr e valu buf1 buf2 store1 store2).
-      assert (Hvv: v1 ~= v2) by eauto.
-      revert Hvv.
-      generalize v1 as x1, v2 as x2.
-      generalize (be_size Hdr_sz l1 l2 (weaken_bit_expr n e)).
-      generalize (be_size Hdr_sz l1 l2 e).
-      intros.
-      inversion Hvv.
-      apply n_tuple_inj in H0.
-      revert Hvv.
-      clear H2 H.
-      revert x1.
-      rewrite H0.
-      intros.
-      rewrite Hvv.
-      auto.
-    - set (v11 := interp_bit_expr (weaken_bit_expr n e1) (valu, bits) buf1 buf2 store1
-                               store2).
-      set (v12 := interp_bit_expr e1 valu buf1 buf2 store1 store2).
-      set (v21 := interp_bit_expr (weaken_bit_expr n e2) (valu, bits) buf1 buf2 store1
-                               store2).
-      set (v22 := interp_bit_expr e2 valu buf1 buf2 store1 store2).
-      assert (Hv1: v11 ~= v12) by eauto.
-      assert (Hv2: v21 ~= v22) by eauto.
-      revert Hv1 Hv2.
-      generalize v11 as x11, v12 as x12.
-      generalize v21 as x21, v22 as x22.
-      generalize (be_size Hdr_sz l1 l2 (weaken_bit_expr n e1)).
-      generalize (be_size Hdr_sz l1 l2 e1).
-      generalize (be_size Hdr_sz l1 l2 (weaken_bit_expr n e2)).
-      generalize (be_size Hdr_sz l1 l2 e2).
-      intros.
-      inversion Hv1.
-      inversion Hv2.
-      clear H2 H H4 H5.
-      apply n_tuple_inj in H0.
-      apply n_tuple_inj in H3.
-      subst n3.
-      subst n1.
-      rewrite Hv1, Hv2.
-      reflexivity.
-  Qed.
-
   Lemma weaken_rel_interp:
     forall c (valu: bval c) n rel (bits: n_tuple bool n) l1 l2 (buf1: n_tuple bool l1) (buf2: n_tuple bool l2) store1 store2,
       interp_store_rel rel valu buf1 buf2 store1 store2 <->
-      interp_store_rel (a:=a) (weaken_store_rel n rel) (valu, bits) buf1 buf2 store1 store2.
+      interp_store_rel (a:=a) (weaken_store_rel a n rel) (valu, bits) buf1 buf2 store1 store2.
   Proof.
     induction rel; intros; simpl; autorewrite with interp_store_rel in *.
     - split; auto.
@@ -2535,6 +2497,11 @@ Section WPProofs.
       intuition eauto.
     - rewrite IHrel1, IHrel2 by eauto.
       intuition eauto.
+    - intuition.
+      print 
+      rewrite IHrel by eauto.
+      intuition eauto.
+    - 
   Qed.
 
   Lemma leap_size_read_bound1:
